thys/MFODL_Monitor_Devel/Monitor_Impl.thy
@@ -8,6 +8,617 @@ theory Monitor_Impl
 begin
 (*>*)
 
+section \<open>Data refinement\<close>
+
+typedef 'a mbuf_t = "UNIV :: 'a list set" ..
+
+setup_lifting type_definition_mbuf_t
+
+instantiation mbuf_t :: (type) size
+begin
+
+lift_definition size_mbuf_t :: "'a mbuf_t \<Rightarrow> nat" is "length" .
+
+instance ..
+
+end
+
+lift_definition mbuf_t_empty :: "'a mbuf_t" is "[]" .
+
+lift_definition mbuf_t_is_empty :: "'a mbuf_t \<Rightarrow> bool" is "\<lambda>xs. xs = []" .
+
+lift_definition mbuf_t_Cons :: "'a \<Rightarrow> 'a mbuf_t \<Rightarrow> 'a mbuf_t" is Cons .
+
+no_notation SCons (infixr "##" 65)
+notation mbuf_t_Cons (infixr "##" 65)
+
+lift_definition mbuf_t_append :: "'a mbuf_t \<Rightarrow> 'a list \<Rightarrow> 'a mbuf_t" is append .
+
+notation mbuf_t_append (infixr "@@" 65)
+
+lift_definition mbuf_t_cases :: "'a mbuf_t \<Rightarrow> 'a option \<times> 'a mbuf_t" is
+  "\<lambda>xs. case xs of [] \<Rightarrow> (None, xs) | y # ys \<Rightarrow> (Some y, ys)" .
+
+lemma Rep_mbuf_t_cases[simp]:
+  "mbuf_t_cases xs = (None, xs') \<Longrightarrow> Rep_mbuf_t xs = []"
+  "mbuf_t_cases xs = (None, xs') \<Longrightarrow> Rep_mbuf_t xs' = []"
+  "mbuf_t_cases xs = (Some x, xs') \<Longrightarrow> Rep_mbuf_t xs = x # Rep_mbuf_t xs'"
+  subgoal by transfer (auto split: option.splits list.splits)
+  subgoal by transfer (auto split: option.splits list.splits)
+  subgoal by transfer (auto split: option.splits list.splits)
+  done
+
+lemma mbuf_t_cases_size[termination_simp]: "(Some x, xs') = mbuf_t_cases xs \<Longrightarrow> size xs' < size xs"
+  by transfer (auto split: list.splits)
+
+lift_definition MBuf2_t :: "'a queue \<Rightarrow> 'a mbuf_t" is "linearize" .
+
+code_datatype MBuf2_t
+
+declare MBuf2_t.rep_eq[code]
+
+lemma mbuf_t_empty_code[code]: "mbuf_t_empty = MBuf2_t empty_queue"
+  by transfer' (auto simp: empty_queue_rep)
+
+lemma mbuf_t_is_empty_code[code]: "mbuf_t_is_empty (MBuf2_t xs) = is_empty xs"
+  by transfer' (auto simp: is_empty_alt)
+
+lemma mbuf_t_Cons_code[code]: "mbuf_t_Cons x (MBuf2_t xs) = MBuf2_t (prepend_queue x xs)"
+  by transfer' (auto simp: prepend_queue_rep)
+
+lemma mbuf_t_append_code[code]: "mbuf_t_append (MBuf2_t xs) ys = MBuf2_t (fold append_queue ys xs)"
+  apply transfer'
+  subgoal for xs ys
+  proof (induction ys arbitrary: xs)
+    case (Cons y ys)
+    show ?case
+      using Cons[of "append_queue y xs"]
+      by (auto simp: append_queue_rep)
+  qed simp
+  done
+
+lemma mbuf_t_cases_code[code]: "mbuf_t_cases (MBuf2_t xs) = (case safe_hd xs of (None, xs') \<Rightarrow> (None, MBuf2_t xs')
+  | (Some x, xs') \<Rightarrow> (Some x, MBuf2_t (tl_queue xs')))"
+  by transfer' (auto simp: tl_queue_rep[unfolded is_empty_alt, OF list.discI] split: list.splits prod.splits option.splits dest: safe_hd_rep)
+
+type_synonym 'a mebuf2 = "'a table mbuf_t \<times> 'a table mbuf_t"
+type_synonym 'a mebufn = "'a table mbuf_t list"
+type_synonym 'a mebuf2S = "'a table mbuf_t \<times> 'a table mbuf_t \<times> ts mbuf_t \<times> bool"
+
+datatype (dead 'msaux, dead 'muaux) meformula =
+  MRel "event_data table"
+  | MPred Formula.name "Formula.trm list" pred_mode
+  | MLet Formula.name nat "('msaux, 'muaux) meformula" "('msaux, 'muaux) meformula"
+  | MLetPast Formula.name nat "('msaux, 'muaux) meformula" "('msaux, 'muaux) meformula" nat "event_data table option"
+  | MAnd "nat set" "('msaux, 'muaux) meformula" bool "nat set" "('msaux, 'muaux) meformula" "event_data mebuf2"
+  | MAndAssign "('msaux, 'muaux) meformula" "nat \<times> Formula.trm"
+  | MAndRel "('msaux, 'muaux) meformula" "Formula.trm \<times> bool \<times> mconstraint \<times> Formula.trm"
+  | MAnds "nat set list" "nat set list" "('msaux, 'muaux) meformula list" "event_data mebufn"
+  | MOr "('msaux, 'muaux) meformula" "('msaux, 'muaux) meformula" "event_data mebuf2"
+  | MNeg "('msaux, 'muaux) meformula"
+  | MExists "('msaux, 'muaux) meformula"
+  | MAgg bool nat Formula.agg_op nat "Formula.trm" "('msaux, 'muaux) meformula"
+  | MPrev \<I> "('msaux, 'muaux) meformula" bool "event_data table mbuf_t" "ts mbuf_t"
+  | MNext \<I> "('msaux, 'muaux) meformula" bool "ts mbuf_t"
+  | MSince args "('msaux, 'muaux) meformula" "('msaux, 'muaux) meformula" "event_data mebuf2S" "'msaux"
+  | MUntil args "('msaux, 'muaux) meformula" "('msaux, 'muaux) meformula" "event_data mebuf2" "ts mbuf_t" ts "'muaux"
+  | MMatchP \<I> "mregex" "mregex list" "('msaux, 'muaux) meformula list" "event_data mebufn" "ts mbuf_t" "event_data mr\<delta>aux"
+  | MMatchF \<I> "mregex" "mregex list" "('msaux, 'muaux) meformula list" "event_data mebufn" "ts mbuf_t" ts "event_data ml\<delta>aux"
+
+fun Rep_meformula :: "('msaux, 'muaux) meformula \<Rightarrow> ('msaux, 'muaux) mformula" where
+  "Rep_meformula (MRel rel) = mformula.MRel rel"
+| "Rep_meformula (MPred e tms mode) = mformula.MPred e tms mode"
+| "Rep_meformula (MLet p m \<phi> \<psi>) = mformula.MLet p m (Rep_meformula \<phi>) (Rep_meformula \<psi>)"
+| "Rep_meformula (MLetPast p m \<phi> \<psi> i buf) = mformula.MLetPast p m (Rep_meformula \<phi>) (Rep_meformula \<psi>) i buf"
+| "Rep_meformula (MAnd A_\<phi> \<phi> pos A_\<psi> \<psi> buf) = mformula.MAnd A_\<phi> (Rep_meformula \<phi>) pos A_\<psi> (Rep_meformula \<psi>) (map_prod Rep_mbuf_t Rep_mbuf_t buf)"
+| "Rep_meformula (MAndAssign \<phi> conf) = mformula.MAndAssign (Rep_meformula \<phi>) conf"
+| "Rep_meformula (MAndRel \<phi> conf) = mformula.MAndRel (Rep_meformula \<phi>) conf"
+| "Rep_meformula (MAnds A_pos A_neg L buf) = mformula.MAnds A_pos A_neg (map Rep_meformula L) (map Rep_mbuf_t buf)"
+| "Rep_meformula (MOr \<phi> \<psi> buf) = mformula.MOr (Rep_meformula \<phi>) (Rep_meformula \<psi>) (map_prod Rep_mbuf_t Rep_mbuf_t buf)"
+| "Rep_meformula (MNeg \<phi>) = mformula.MNeg (Rep_meformula \<phi>)"
+| "Rep_meformula (MExists \<phi>) = mformula.MExists (Rep_meformula \<phi>)"
+| "Rep_meformula (MAgg g0 y \<omega> b f \<phi>) = mformula.MAgg g0 y \<omega> b f (Rep_meformula \<phi>)"
+| "Rep_meformula (MPrev I \<phi> first buf nts) = mformula.MPrev I (Rep_meformula \<phi>) first (Rep_mbuf_t buf) (Rep_mbuf_t nts)"
+| "Rep_meformula (MNext I \<phi> first nts) = mformula.MNext I (Rep_meformula \<phi>) first (Rep_mbuf_t nts)"
+| "Rep_meformula (MSince args \<phi> \<psi> buf aux) = mformula.MSince args (Rep_meformula \<phi>) (Rep_meformula \<psi>)
+    (case buf of (a, b, c, d) \<Rightarrow> (Rep_mbuf_t a, Rep_mbuf_t b, Rep_mbuf_t c, d)) aux"
+| "Rep_meformula (MUntil args \<phi> \<psi> buf nts t aux) = mformula.MUntil args (Rep_meformula \<phi>) (Rep_meformula \<psi>)
+    (map_prod Rep_mbuf_t Rep_mbuf_t buf) (Rep_mbuf_t nts) t aux"
+| "Rep_meformula (MMatchP I mr mrs \<phi>s buf nts aux) = mformula.MMatchP I mr mrs (map Rep_meformula \<phi>s)
+    (map Rep_mbuf_t buf) (Rep_mbuf_t nts) aux"
+| "Rep_meformula (MMatchF I mr mrs \<phi>s buf nts t aux) = mformula.MMatchF I mr mrs (map Rep_meformula \<phi>s)
+    (map Rep_mbuf_t buf) (Rep_mbuf_t nts) t aux"
+
+lemma size_list_cong: "xs = ys \<Longrightarrow> (\<And>x. x \<in> set xs \<Longrightarrow> f x = g x) \<Longrightarrow> size_list f xs = size_list g ys"
+  by (induct xs arbitrary: ys) auto
+
+lemma size_Rep_meformula[simp]: "size (Rep_meformula \<psi>) = size \<psi>"
+  by (induction \<psi> rule: Rep_meformula.induct) (auto simp: comp_def cong: size_list_cong)
+
+code_datatype Rep_meformula
+
+abbreviation (input) "init_mebuf2S \<equiv> (mbuf_t_empty, mbuf_t_empty, mbuf_t_empty, False)"
+
+function (in maux) (sequential) meinit0 :: "nat \<Rightarrow> Formula.formula \<Rightarrow> ('msaux, 'muaux) meformula" where
+  "meinit0 n (Formula.Neg \<phi>) = (if fv \<phi> = {} then MNeg (meinit0 n \<phi>) else MRel empty_table)"
+| "meinit0 n (Formula.Eq t1 t2) = MRel (eq_rel n t1 t2)"
+| "meinit0 n (Formula.Pred e ts) = MPred e ts (pred_mode_of n ts)"
+| "meinit0 n (Formula.Let p \<phi> \<psi>) = MLet p (Formula.nfv \<phi>) (meinit0 (Formula.nfv \<phi>) \<phi>) (meinit0 n \<psi>)"
+| "meinit0 n (Formula.LetPast p \<phi> \<psi>) = MLetPast p (Formula.nfv \<phi>) (meinit0 (Formula.nfv \<phi>) \<phi>) (meinit0 n \<psi>) 0 None"
+| "meinit0 n (Formula.Or \<phi> \<psi>) = MOr (meinit0 n \<phi>) (meinit0 n \<psi>) (mbuf_t_empty, mbuf_t_empty)"
+| "meinit0 n (Formula.And \<phi> \<psi>) = (if safe_assignment (fv \<phi>) \<psi> then
+      MAndAssign (meinit0 n \<phi>) (split_assignment (fv \<phi>) \<psi>)
+    else if safe_formula \<psi> then
+      MAnd (fv \<phi>) (meinit0 n \<phi>) True (fv \<psi>) (meinit0 n \<psi>) (mbuf_t_empty, mbuf_t_empty)
+    else if is_constraint \<psi> then
+      MAndRel (meinit0 n \<phi>) (split_constraint \<psi>)
+    else (case \<psi> of Formula.Neg \<psi> \<Rightarrow>
+      MAnd (fv \<phi>) (meinit0 n \<phi>) False (fv \<psi>) (meinit0 n \<psi>) (mbuf_t_empty, mbuf_t_empty)
+      | _ \<Rightarrow> MRel empty_table))"
+| "meinit0 n (Formula.Ands l) = (let (pos, neg) = partition safe_formula l in
+    let mpos = map (meinit0 n) pos in
+    let mneg = map (meinit0 n) (map remove_neg neg) in
+    let vpos = map fv pos in
+    let vneg = map fv neg in
+    MAnds vpos vneg (mpos @ mneg) (replicate (length l) mbuf_t_empty))"
+| "meinit0 n (Formula.Exists \<phi>) = MExists (meinit0 (Suc n) \<phi>)"
+| "meinit0 n (Formula.Agg y \<omega> b f \<phi>) = MAgg (fv \<phi> \<subseteq> {0..<b}) y \<omega> b f (meinit0 (b + n) \<phi>)"
+| "meinit0 n (Formula.Prev I \<phi>) = MPrev I (meinit0 n \<phi>) True mbuf_t_empty mbuf_t_empty"
+| "meinit0 n (Formula.Next I \<phi>) = MNext I (meinit0 n \<phi>) True mbuf_t_empty"
+| "meinit0 n (Formula.Since \<phi> I \<psi>) = (if safe_formula \<phi>
+    then MSince (init_args I n (Formula.fv \<phi>) (Formula.fv \<psi>) True) (meinit0 n \<phi>) (meinit0 n \<psi>) init_mebuf2S (init_msaux (init_args I n (Formula.fv \<phi>) (Formula.fv \<psi>) True))
+    else (case \<phi> of
+      Formula.Neg \<phi> \<Rightarrow> MSince (init_args I n (Formula.fv \<phi>) (Formula.fv \<psi>) False) (meinit0 n \<phi>) (meinit0 n \<psi>) init_mebuf2S (init_msaux (init_args I n (Formula.fv \<phi>) (Formula.fv \<psi>) False))
+    | _ \<Rightarrow> MRel empty_table))"
+| "meinit0 n (Formula.Until \<phi> I \<psi>) = (if safe_formula \<phi>
+    then MUntil (init_args I n (Formula.fv \<phi>) (Formula.fv \<psi>) True) (meinit0 n \<phi>) (meinit0 n \<psi>) (mbuf_t_empty, mbuf_t_empty) mbuf_t_empty 0 (init_muaux (init_args I n (Formula.fv \<phi>) (Formula.fv \<psi>) True))
+    else (case \<phi> of
+      Formula.Neg \<phi> \<Rightarrow> MUntil (init_args I n (Formula.fv \<phi>) (Formula.fv \<psi>) False) (meinit0 n \<phi>) (meinit0 n \<psi>) (mbuf_t_empty, mbuf_t_empty) mbuf_t_empty 0 (init_muaux (init_args I n (Formula.fv \<phi>) (Formula.fv \<psi>) False))
+    | _ \<Rightarrow> MRel empty_table))"
+| "meinit0 n (Formula.MatchP I r) =
+    (let (mr, \<phi>s) = to_mregex r
+    in MMatchP I mr (sorted_list_of_set (RPDs mr)) (map (meinit0 n) \<phi>s) (replicate (length \<phi>s) mbuf_t_empty) mbuf_t_empty [])"
+| "meinit0 n (Formula.MatchF I r) =
+    (let (mr, \<phi>s) = to_mregex r
+    in MMatchF I mr (sorted_list_of_set (LPDs mr)) (map (meinit0 n) \<phi>s) (replicate (length \<phi>s) mbuf_t_empty) mbuf_t_empty 0 [])"
+| "meinit0 n _ = MRel empty_table"
+  by pat_completeness auto
+termination (in maux)
+  by (relation "measure (\<lambda>(_, \<phi>). size \<phi>)")
+    (auto simp: less_Suc_eq_le size_list_estimation' size_remove_neg
+      dest!: to_mregex_ok[OF sym] atms_size)
+
+lemma (in maux) minit0_code[code]: "minit0 n \<phi> = Rep_meformula (meinit0 n \<phi>)"
+  by (induction n \<phi> rule: meinit0.induct) (auto simp: mbuf_t_empty.rep_eq split: formula.splits prod.splits)
+
+lemma (in maux) minit_code[code]: "minit \<phi> = (let n = Formula.nfv \<phi> in \<lparr>mstate_i = 0, mstate_j = 0, mstate_m = Rep_meformula (meinit0 n \<phi>), mstate_n = n\<rparr>)"
+  by (auto simp: minit_def Let_def minit0_code)
+
+fun meprev_next :: "\<I> \<Rightarrow> event_data table mbuf_t \<Rightarrow> ts mbuf_t \<Rightarrow> event_data table list \<times> event_data table mbuf_t \<times> ts mbuf_t" where
+  "meprev_next I xs ts = (case mbuf_t_cases xs of (None, xs') \<Rightarrow> ([], mbuf_t_empty, ts)
+  | (Some x, xs') \<Rightarrow> (case mbuf_t_cases ts of (None, ts') \<Rightarrow> ([], x ## xs', mbuf_t_empty)
+  | (Some t, ts') \<Rightarrow> (case mbuf_t_cases ts' of (None, ts'') \<Rightarrow> ([], x ## xs', t ## mbuf_t_empty)
+  | (Some t', ts'') \<Rightarrow> (let (ys, zs) = meprev_next I xs' (t' ## ts'')
+    in ((if mem I ((t' - t)) then x else empty_table) # ys, zs)))))"
+
+lemma meprev_next: "meprev_next I xs ts = (zs, xs', ts') \<Longrightarrow> mprev_next I (Rep_mbuf_t xs) (Rep_mbuf_t ts) =
+  (zs, Rep_mbuf_t xs', Rep_mbuf_t ts')"
+proof (induction I xs ts arbitrary: zs xs' ts' rule: meprev_next.induct)
+  case (1 I xs ts)
+  obtain xo xs'' where xs_def: "mbuf_t_cases xs = (xo, xs'')"
+    by fastforce
+  obtain to ts'' where ts_def: "mbuf_t_cases ts = (to, ts'')"
+    by fastforce
+  obtain to' ts''' where ts''_def: "mbuf_t_cases ts'' = (to', ts''')"
+    by fastforce
+  show ?case
+    using 1
+    by (cases xo; cases to; cases to')
+       (auto simp: xs_def ts_def ts''_def mbuf_t_empty.rep_eq mbuf_t_Cons.rep_eq split: prod.splits)
+qed
+
+fun mebuf2_add :: "event_data table list \<Rightarrow> event_data table list \<Rightarrow> event_data mebuf2 \<Rightarrow> event_data mebuf2" where
+  "mebuf2_add xs' ys' (xs, ys) = (xs @@ xs', ys @@ ys')"
+
+lemma mbuf2_add: "mbuf2_add xs ys (map_prod Rep_mbuf_t Rep_mbuf_t buf) = map_prod Rep_mbuf_t Rep_mbuf_t (mebuf2_add xs ys buf)"
+  by (cases buf) (auto simp: mbuf_t_append.rep_eq)
+
+fun mebuf2S_add :: "event_data table list \<Rightarrow> event_data table list \<Rightarrow> ts list \<Rightarrow> event_data mebuf2S \<Rightarrow> event_data mebuf2S" where
+  "mebuf2S_add xs' ys' ts' (xs, ys, ts, skew) = (xs @@ xs', ys @@ ys', ts @@ ts', skew)"
+
+fun mebuf2_take :: "(event_data table \<Rightarrow> event_data table \<Rightarrow> 'b) \<Rightarrow> event_data mebuf2 \<Rightarrow> 'b list \<times> event_data mebuf2" where
+  "mebuf2_take f (xs, ys) = (case mbuf_t_cases xs of (None, xs') \<Rightarrow> ([], (xs', ys)) | (Some x, xs') \<Rightarrow>
+    (case mbuf_t_cases ys of (None, ys') \<Rightarrow> ([], (x ## xs', ys')) | (Some y, ys') \<Rightarrow>
+    let (zs, buf) = mebuf2_take f (xs', ys') in (f x y # zs, buf)))"
+
+lemma mebuf2_take_aux: "mebuf2_take f (xs, ys) = (zs, (xs', ys')) \<Longrightarrow>
+  mbuf2_take f (Rep_mbuf_t xs, Rep_mbuf_t ys) = (zs, (Rep_mbuf_t xs', Rep_mbuf_t ys'))"
+proof (induction f "(xs, ys)" arbitrary: xs ys zs xs' ys' rule: mebuf2_take.induct)
+  case (1 f xs ys)
+  obtain x xs'' where xs_def: "mbuf_t_cases xs = (x, xs'')"
+    by fastforce
+  obtain y ys'' where ys_def: "mbuf_t_cases ys = (y, ys'')"
+    by fastforce
+  show ?case
+    using 1 xs_def ys_def
+    by (cases x; cases y) (auto simp: mbuf_t_Cons.rep_eq split: prod.splits)
+qed
+
+lemma mebuf2_take: "mebuf2_take f buf = (zs, buf') \<Longrightarrow>
+  mbuf2_take f (map_prod Rep_mbuf_t Rep_mbuf_t buf) = (zs, (map_prod Rep_mbuf_t Rep_mbuf_t buf'))"
+  using mebuf2_take_aux
+  by (cases buf; cases buf') fastforce
+
+fun mebuf2t_take :: "(event_data table \<Rightarrow> event_data table \<Rightarrow> ts \<Rightarrow> 'b \<Rightarrow> 'b) \<Rightarrow> 'b \<Rightarrow>
+    event_data mebuf2 \<Rightarrow> ts \<Rightarrow> ts mbuf_t \<Rightarrow> 'b \<times> event_data mebuf2 \<times> ts \<times> ts mbuf_t" where
+  "mebuf2t_take f z (xs, ys) t0 ts =
+    (case mbuf_t_cases ts of (None, ts') \<Rightarrow> (z, (xs, ys), t0, ts') | (Some t, ts') \<Rightarrow>
+    (case mbuf_t_cases xs of (None, xs') \<Rightarrow> (z, (xs', ys), t, t ## ts') | (Some x, xs') \<Rightarrow>
+    (case mbuf_t_cases ys of (None, ys') \<Rightarrow> (z, (x ## xs', ys'), t, t ## ts') | (Some y, ys') \<Rightarrow>
+    mebuf2t_take f (f x y t z) (xs', ys') t ts')))"
+
+lemma mebuf2t_take_aux: "mebuf2t_take f z (xs, ys) t ts = (zs, (xs', ys'), nt, ts') \<Longrightarrow>
+  mbuf2t_take f z (Rep_mbuf_t xs, Rep_mbuf_t ys) t (Rep_mbuf_t ts) = (zs, (Rep_mbuf_t xs', Rep_mbuf_t ys'), nt, Rep_mbuf_t ts')"
+proof (induction f z "(xs, ys)" t ts arbitrary: xs ys rule: mebuf2t_take.induct)
+  case (1 f z xs ys t ts)
+  obtain x xs'' where xs_def: "mbuf_t_cases xs = (x, xs'')"
+    by fastforce
+  obtain y ys'' where ys_def: "mbuf_t_cases ys = (y, ys'')"
+    by fastforce
+  obtain t ts'' where ts_def: "mbuf_t_cases ts = (t, ts'')"
+    by fastforce
+  show ?case
+    using 1 xs_def ys_def ts_def
+    by (cases x; cases y; cases t) (auto simp: mbuf_t_Cons.rep_eq split: prod.splits list.splits)
+qed
+
+lemma mebuf2t_take: "mebuf2t_take f z buf t ts = (zs, buf', nt, nts) \<Longrightarrow>
+  mbuf2t_take f z (map_prod Rep_mbuf_t Rep_mbuf_t buf) t (Rep_mbuf_t ts) = (zs, (map_prod Rep_mbuf_t Rep_mbuf_t buf'), nt, Rep_mbuf_t nts)"
+  using mebuf2t_take_aux
+  by (cases buf; cases buf') fastforce
+
+context maux begin
+context fixes args :: args begin
+
+fun eeval_since :: "event_data table list \<Rightarrow> event_data mebuf2S \<Rightarrow> 'msaux \<Rightarrow>
+  event_data table list \<times> event_data mebuf2S \<times> 'msaux" where
+  "eeval_since rs (xs, ys, ts, skew) aux =
+    (case mbuf_t_cases ys of (None, ys') \<Rightarrow>
+      (case mbuf_t_cases xs of (Some x, xs') \<Rightarrow>
+        (case mbuf_t_cases ts of (Some t, ts') \<Rightarrow>
+    (if skew \<or> memL (args_ivl args) 0
+    then (rev rs, (x ## xs', mbuf_t_empty, t ## ts', skew), aux)
+    else (let aux' = join_msaux args x (add_new_ts_msaux args t aux)
+      in (rev (result_msaux args aux' # rs), (xs', mbuf_t_empty, ts', True), aux')))
+        | (None, ts') \<Rightarrow> (rev rs, (x ## xs', mbuf_t_empty, mbuf_t_empty, skew), aux))
+      | (None, xs') \<Rightarrow> (rev rs, (mbuf_t_empty, mbuf_t_empty, ts, skew), aux))
+    | (Some y, ys') \<Rightarrow>
+      if skew then eeval_since rs (xs, ys', ts, False) (add_new_table_msaux args y aux) else
+      (case mbuf_t_cases xs of (Some x, xs') \<Rightarrow>
+        (case mbuf_t_cases ts of (Some t, ts') \<Rightarrow>
+    (let aux' = add_new_table_msaux args y (join_msaux args x (add_new_ts_msaux args t aux))
+    in eeval_since (result_msaux args aux' # rs) (xs', ys', ts', False) aux')
+        | (None, ts') \<Rightarrow> (rev rs, (x ## xs', y ## ys', ts', skew), aux))
+      | (None, xs') \<Rightarrow> (rev rs, (mbuf_t_empty, y ## ys', ts, skew), aux)))"
+
+lemma eeval_since: "eeval_since rs (xs, ys, ts, skew) aux = (res, (xs', ys', ts', skew'), aux') \<Longrightarrow>
+  eval_since args rs (Rep_mbuf_t xs, Rep_mbuf_t ys, Rep_mbuf_t ts, skew) aux = (res, (Rep_mbuf_t xs', Rep_mbuf_t ys', Rep_mbuf_t ts', skew'), aux')"
+proof (induction rs "(xs, ys, ts, skew)" aux arbitrary: xs ys ts skew res xs' ys' ts' skew' aux' rule: eeval_since.induct)
+  case (1 rs xs ys ts skew aux)
+  obtain x xs'' where xs_def: "mbuf_t_cases xs = (x, xs'')"
+    by fastforce
+  obtain y ys'' where ys_def: "mbuf_t_cases ys = (y, ys'')"
+    by fastforce
+  obtain t ts'' where ts_def: "mbuf_t_cases ts = (t, ts'')"
+    by fastforce
+  show ?case
+    using 1 xs_def ys_def ts_def
+    by (cases x; cases y; cases t) (auto simp: mbuf_t_empty.rep_eq mbuf_t_Cons.rep_eq Let_def split: if_splits)
+qed
+
+end (* fixes args *)
+end (* maux *)
+
+fun mebufn_add :: "event_data table list list \<Rightarrow> event_data mebufn \<Rightarrow> event_data mebufn" where
+  "mebufn_add xs' xs = List.map2 (@@) xs xs'"
+
+lemma mbufn_add: "mbufn_add xss (map Rep_mbuf_t buf) = map Rep_mbuf_t (mebufn_add xss buf)"
+  by (auto simp: comp_def zip_map1 mbuf_t_append.rep_eq)
+
+lemma size_snd_mbuf_t_cases: "\<not> mbuf_t_is_empty a \<Longrightarrow> size (snd (mbuf_t_cases a)) < size a"
+  by transfer (auto split: list.splits)
+
+lemma size_list_snd_mbuf_t_cases: assumes "buf \<noteq> []" "\<And>x. x \<in> set buf \<Longrightarrow> \<not> mbuf_t_is_empty x"
+  shows "size_list (\<lambda>x. size (snd (mbuf_t_cases x))) buf < size_list size buf"
+  using assms
+proof (induction buf)
+  case IH: (Cons a buf)
+  show ?case
+  proof (cases buf)
+    case Nil
+    show ?thesis
+      using IH(3) size_snd_mbuf_t_cases
+      by (auto simp: Nil)
+  next
+    case (Cons a' buf')
+    have "size_list (\<lambda>x. size (snd (mbuf_t_cases x))) buf < size_list size buf"
+      using IH(1,3)
+      by (auto simp: Cons)
+    then show ?thesis
+      using IH(3) size_snd_mbuf_t_cases
+      by force
+  qed
+qed auto
+
+function mebufn_take :: "(event_data table list \<Rightarrow> 'b \<Rightarrow> 'b) \<Rightarrow> 'b \<Rightarrow> event_data mebufn \<Rightarrow> 'b \<times> event_data mebufn" where
+  "mebufn_take f z buf = (if buf = [] \<or> (\<exists>x \<in> set buf. mbuf_t_is_empty x) then (z, buf)
+    else mebufn_take f (f (map (the \<circ> fst \<circ> mbuf_t_cases) buf) z) (map (snd \<circ> mbuf_t_cases) buf))"
+  by pat_completeness auto
+termination
+  using size_list_snd_mbuf_t_cases
+  by (relation "measure (\<lambda>(_, _, buf). size_list size buf)") (auto simp: comp_def Suc_le_eq size_list_length_diff1)
+
+lemma mbuf_t_is_empty_in_set: "[] \<in> set (map Rep_mbuf_t buf) \<longleftrightarrow> (\<exists>x \<in> set buf. mbuf_t_is_empty x)"
+  by transfer auto
+
+lemma hd_Rep_mbuf_t:
+  assumes "\<And>x. x \<in> set buf \<Longrightarrow> \<not> mbuf_t_is_empty x"
+  shows "map (hd \<circ> Rep_mbuf_t) buf = map (the \<circ> fst \<circ> mbuf_t_cases) buf"
+  using assms
+  by transfer (auto split: list.splits)
+
+lemma tl_Rep_mbuf_t:
+  assumes "\<And>x. x \<in> set buf \<Longrightarrow> \<not> mbuf_t_is_empty x"
+  shows "map (tl \<circ> Rep_mbuf_t) buf = map Rep_mbuf_t (map (snd \<circ> mbuf_t_cases) buf)"
+  using assms
+  by transfer (auto split: list.splits)
+
+lemma mebufn_take: "mebufn_take f z buf = (z', buf') \<Longrightarrow>
+  mbufn_take f z (map Rep_mbuf_t buf) = (z', map Rep_mbuf_t buf')"
+proof (induction f z buf arbitrary: z' buf' rule: mebufn_take.induct)
+  case (1 f z buf)
+  show ?case
+    using 1(1,2)
+    unfolding mebufn_take.simps[of _ _ buf] mbufn_take.simps[of _ _ "map Rep_mbuf_t buf"] mbuf_t_is_empty_in_set map_is_Nil_conv
+    by (auto simp del: mbufn_take.simps mebufn_take.simps simp: hd_Rep_mbuf_t tl_Rep_mbuf_t split: if_splits)
+qed
+
+lemma mbufn_take_app: "mbufn_take (\<lambda>xs zs. zs @@ [f xs]) zs buf = (buf', zs') \<Longrightarrow>
+  mbufn_take (\<lambda>xs zs. zs @ [f xs]) (Rep_mbuf_t zs) buf = (buf'', zs'') \<Longrightarrow>
+  buf'' = Rep_mbuf_t buf' \<and> zs'' = zs'"
+proof (induction "\<lambda>xs zs. zs @@ [f xs]" zs buf rule: mbufn_take.induct)
+  case (1 z buf)
+  then show ?case
+    by (auto simp: mbufn_take.simps[where ?buf="buf"] mbuf_t_append.rep_eq simp del: mbufn_take.simps split: if_splits)
+qed
+
+fun mebufnt_take :: "(event_data table list \<Rightarrow> ts \<Rightarrow> 'b \<Rightarrow> 'b) \<Rightarrow>
+    'b \<Rightarrow> event_data mebufn \<Rightarrow> ts \<Rightarrow> ts mbuf_t \<Rightarrow> 'b \<times> event_data mebufn \<times> ts \<times> ts mbuf_t" where
+  "mebufnt_take f z buf t0 ts =
+    (case mbuf_t_cases ts of (None, ts') \<Rightarrow> (z, buf, t0, ts) | (Some t, ts') \<Rightarrow>
+    (if (\<exists>x \<in> set buf. mbuf_t_is_empty x) then (z, buf, t, t ## ts')
+    else mebufnt_take f (f (map (the \<circ> fst \<circ> mbuf_t_cases) buf) t z) (map (snd \<circ> mbuf_t_cases) buf) t ts'))"
+
+lemma mebufnt_take: "mebufnt_take f z buf t nts = (z', buf', nt, nts') \<Longrightarrow>
+  mbufnt_take f z (map Rep_mbuf_t buf) t (Rep_mbuf_t nts) = (z', map Rep_mbuf_t buf', nt, Rep_mbuf_t nts')"
+proof (induction f z buf t nts arbitrary: z' buf' nts' rule: mebufnt_take.induct)
+  case (1 f z buf t ts)
+  obtain to ts'' where ts_def: "mbuf_t_cases ts = (to, ts'')"
+    by fastforce
+  show ?case
+    using 1(1,2) ts_def
+    unfolding mebufnt_take.simps[of _ _ buf] mbufnt_take.simps[of _ _ "map Rep_mbuf_t buf"] mbuf_t_is_empty_in_set map_is_Nil_conv
+    by (cases to) (auto simp del: mbufnt_take.simps mebufnt_take.simps simp: hd_Rep_mbuf_t tl_Rep_mbuf_t mbuf_t_Cons.rep_eq split: if_splits)
+qed
+
+lemma mbufnt_take_app: "mbufnt_take (\<lambda>xs t (zs, aux). case f xs t aux of (z, aux) \<Rightarrow> (zs @@ [z], aux)) (zs, aux) buf t0 ts = ((zs', aux'), buf', nt', ts') \<Longrightarrow>
+  mbufnt_take (\<lambda>xs t (zs, aux). case f xs t aux of (z, aux) \<Rightarrow> (zs @ [z], aux)) (Rep_mbuf_t zs, aux) buf t0 ts = ((zs'', aux''), buf'', nt'', ts'') \<Longrightarrow>
+  zs'' = Rep_mbuf_t zs' \<and> aux'' = aux' \<and> buf'' = buf' \<and> nt'' = nt' \<and> ts'' = ts'"
+proof (induction "\<lambda>xs t (zs, aux). case f xs t aux of (z, aux) \<Rightarrow> (zs @@ [z], aux)" "(zs, aux)" buf t0 ts arbitrary: zs aux rule: mbufnt_take.induct)
+  case (1 buf t0 ts)
+  then show ?case
+    by (auto simp: mbufnt_take.simps[where ?ts=ts] mbuf_t_append.rep_eq simp del: mbufnt_take.simps split: if_splits prod.splits)
+qed
+
+function letpast_meeval0 where
+  "letpast_meeval0 eval j i ys xs p ts db \<phi> =
+     (let (ys', \<phi>') = eval ts (Mapping.update p xs db) \<phi>
+     in if size \<phi>' \<noteq> size \<phi> then (mbuf_t_empty, 0, None, \<phi>)
+     else (case ys' of
+       [] \<Rightarrow> (ys @@ ys', i + length xs, None, \<phi>')
+     | y # _ \<Rightarrow> (if Suc (i + length xs) \<ge> j then (ys @@ ys', i + length xs, Some y, \<phi>')
+         else letpast_meeval0 eval j (i + length xs) (ys @@ ys') ys' p [] (Mapping.map_values (\<lambda>_ _. []) db) \<phi>')))"
+  by auto
+termination
+  by (relation "measure (\<lambda>(_, j, i, _, xs, _). j - (i + length xs))")
+    (auto simp: not_le min_def diff_less_mono2)
+
+declare letpast_meeval0.simps[simp del]
+
+lemma letpast_meeval0: "letpast_meeval0 eval j i ys xs p ts db \<phi> = (ys', i', buf', \<phi>') \<Longrightarrow>
+  letpast_meval0 eval j i (Rep_mbuf_t ys) xs p ts db \<phi> = (Rep_mbuf_t ys', i', buf', \<phi>')"
+proof (induction eval j i ys xs p ts db \<phi> rule: letpast_meeval0.induct)
+  case (1 eval j i ys xs p ts db \<phi>)
+  then show ?case
+    by (auto simp: letpast_meeval0.simps[where \<phi>=\<phi>] letpast_meval0.simps[where \<phi>=\<phi>]
+        mbuf_t_empty.rep_eq mbuf_t_append.rep_eq split: prod.splits list.splits)
+qed
+
+lemma letpast_meeval0_cong[fundef_cong]:
+  assumes "(\<And>ts db \<psi>. size \<psi> = size \<phi> \<Longrightarrow>  eval ts db \<psi> = eval' ts db \<psi>)"
+  shows "letpast_meeval0 eval j i ys xs p ts db \<phi> = letpast_meeval0 eval' j i ys xs p ts db \<phi>"
+  using assms
+  apply (induct eval j i ys xs p ts db \<phi> arbitrary: eval' rule: letpast_meeval0.induct)
+  subgoal premises IH for eval j i ys xs p ts db \<phi> eval'
+    apply (subst (1 2) letpast_meeval0.simps)
+    apply (auto split: prod.splits list.splits simp: Let_def IH)
+    done
+  done
+
+lemma size_letpast_meeval: "(\<And>ts db \<psi>. size \<psi> = size \<phi> \<Longrightarrow> size (snd (eval ts db \<psi>)) = size \<psi>) \<Longrightarrow>
+  size (snd (snd (snd (letpast_meeval0 eval j i ys xs p ts db \<phi>)))) = size \<phi>"
+  apply (induct eval j i ys xs p ts db \<phi> rule: letpast_meeval0.induct)
+  apply (subst letpast_meeval0.simps)
+  apply (auto split: prod.splits list.splits simp: Let_def dest: sndI)
+  done
+
+lemma letpast_meval0_cong_f:
+  assumes "(\<And>ts db \<psi>. size \<psi> = size \<phi> \<Longrightarrow>  eval ts db (f \<psi>) = (case eval' ts db \<psi> of (zs, \<psi>') \<Rightarrow> (zs, f \<psi>')))"
+    "\<And>\<psi>. size (f \<psi>) = size \<psi>"
+    "letpast_meval0 eval j i ys xs p ts db (f \<phi>) = (ys', i', buf', \<phi>')"
+    "letpast_meval0 eval' j i ys xs p ts db \<phi> = (ys'', i'', buf'', \<phi>'')"
+  shows "ys' = ys'' \<and> i' = i'' \<and> buf' = buf'' \<and> \<phi>' = f \<phi>''"
+  using assms
+  apply (induct eval' j i ys xs p ts db \<phi> rule: letpast_meval0.induct)
+  subgoal premises IH for eval j i ys xs p ts db \<phi>
+    using IH
+    by (auto simp: letpast_meval0.simps[where ?\<phi>=\<phi>] letpast_meval0.simps[where ?\<phi>="f \<phi>"]
+        split: prod.splits list.splits if_splits simp: Let_def)
+  done
+
+context maux
+begin
+
+context
+  fixes j :: nat
+begin
+
+function (sequential) meeval :: "nat \<Rightarrow> ts list \<Rightarrow> database \<Rightarrow> ('msaux, 'muaux) meformula \<Rightarrow>
+  event_data table list \<times> ('msaux, 'muaux) meformula" where
+  "meeval n ts db (MRel rel) = (replicate (length ts) rel, MRel rel)"
+| "meeval n ts db (MPred e tms mode) =
+    ((case Mapping.lookup db (e, length tms) of
+        None \<Rightarrow> replicate (length ts) {}
+      | Some xs \<Rightarrow> (case mode of
+          Copy \<Rightarrow> xs
+        | Simple \<Rightarrow> map (\<lambda>X. simple_match n 0 tms ` X) xs
+        | Match \<Rightarrow> map (\<lambda>X. (\<lambda>f. Table.tabulate f 0 n) ` Option.these (match tms ` X)) xs)),
+    MPred e tms mode)"
+| "meeval n ts db (MLet p m \<phi> \<psi>) =
+    (let (xs, \<phi>) = meeval m ts db \<phi>;
+      (ys, \<psi>) = meeval n ts (Mapping.update (p, m) xs db) \<psi>
+    in (ys, MLet p m \<phi> \<psi>))"
+| "meeval n ts db (MLetPast p m \<phi> \<psi> i buf) =
+    (let (xs, i, buf, \<phi>) = letpast_meeval0 (meeval m) j i mbuf_t_empty (list_of_option buf) (p, m) ts db \<phi>;
+         (ys, \<psi>) = meeval n ts (Mapping.update (p, m) (Rep_mbuf_t xs) db) \<psi>
+    in (ys, MLetPast p m \<phi> \<psi> i buf))"
+| "meeval n ts db (MAnd A_\<phi> \<phi> pos A_\<psi> \<psi> buf) =
+    (let (xs, \<phi>) = meeval n ts db \<phi>; (ys, \<psi>) = meeval n ts db \<psi>;
+      (zs, buf) = mebuf2_take (\<lambda>r1 r2. bin_join n A_\<phi> r1 pos A_\<psi> r2) (mebuf2_add xs ys buf)
+    in (zs, MAnd A_\<phi> \<phi> pos A_\<psi> \<psi> buf))"
+| "meeval n ts db (MAndAssign \<phi> conf) =
+    (let (xs, \<phi>) = meeval n ts db \<phi> in (map (\<lambda>r. eval_assignment conf ` r) xs, MAndAssign \<phi> conf))"
+| "meeval n ts db (MAndRel \<phi> conf) =
+    (let (xs, \<phi>) = meeval n ts db \<phi> in (map (Set.filter (eval_constraint conf)) xs, MAndRel \<phi> conf))"
+| "meeval n ts db (MAnds A_pos A_neg L buf) =
+    (let R = map (meeval n ts db) L in
+    let buf = mebufn_add (map fst R) buf in
+    let (zs, buf) = mebufn_take (\<lambda>xs zs. zs @@ [mmulti_join n A_pos A_neg xs]) mbuf_t_empty buf in
+    (Rep_mbuf_t zs, MAnds A_pos A_neg (map snd R) buf))"
+| "meeval n ts db (MOr \<phi> \<psi> buf) =
+    (let (xs, \<phi>) = meeval n ts db \<phi>; (ys, \<psi>) = meeval n ts db \<psi>;
+      (zs, buf) = mebuf2_take (\<lambda>r1 r2. r1 \<union> r2) (mebuf2_add xs ys buf)
+    in (zs, MOr \<phi> \<psi> buf))"
+| "meeval n ts db (MNeg \<phi>) =
+    (let (xs, \<phi>) = meeval n ts db \<phi> in (map (\<lambda>r. (if r = empty_table then unit_table n else empty_table)) xs, MNeg \<phi>))"
+| "meeval n ts db (MExists \<phi>) =
+    (let (xs, \<phi>) = meeval (Suc n) ts db \<phi> in (map (\<lambda>r. tl ` r) xs, MExists \<phi>))"
+| "meeval n ts db (MAgg g0 y \<omega> b f \<phi>) =
+    (let (xs, \<phi>) = meeval (b + n) ts db \<phi> in (map (eval_agg n g0 y \<omega> b f) xs, MAgg g0 y \<omega> b f \<phi>))"
+| "meeval n ts db (MPrev I \<phi> first buf nts) =
+    (let (xs, \<phi>) = meeval n ts db \<phi>
+    in if first \<and> ts = [] then ([], MPrev I \<phi> True (buf @@ xs) (nts @@ ts))
+    else let (zs, buf, nts) = meprev_next I (buf @@ xs) (nts @@ ts)
+      in (if first then empty_table # zs else zs, MPrev I \<phi> False buf nts))"
+| "meeval n ts db (MNext I \<phi> first nts) =
+    (let (xs, \<phi>) = meeval n ts db \<phi>;
+      (xs, first) = (case (xs, first) of (_ # xs, True) \<Rightarrow> (xs, False) | a \<Rightarrow> a);
+      (zs, _, nts) = meprev_next I (mbuf_t_empty @@ xs) (nts @@ ts)
+    in (zs, MNext I \<phi> first nts))"
+| "meeval n ts db (MSince args \<phi> \<psi> buf aux) =
+    (let (xs, \<phi>) = meeval n ts db \<phi>; (ys, \<psi>) = meeval n ts db \<psi>;
+      (zs, buf, aux) = eeval_since args [] (mebuf2S_add xs ys ts buf) aux
+    in (zs, MSince args \<phi> \<psi> buf aux))"
+| "meeval n ts db (MUntil args \<phi> \<psi> buf nts t aux) =
+    (let (xs, \<phi>) = meeval n ts db \<phi>; (ys, \<psi>) = meeval n ts db \<psi>;
+      (aux, buf, nt, nts') = mebuf2t_take (add_new_muaux args) aux (mebuf2_add xs ys buf) t (nts @@ ts);
+      (zs, aux) = eval_muaux args nt aux
+    in (zs, MUntil args \<phi> \<psi> buf nts' nt aux))"
+| "meeval n ts db (MMatchP I mr mrs \<phi>s buf nts aux) =
+    (let (xss, \<phi>s) = map_split id (map (meeval n ts db) \<phi>s);
+      ((zs, aux), buf, _, nts) = mebufnt_take (\<lambda>rels t (zs, aux).
+        let (z, aux) = update_matchP n I mr mrs rels t aux
+        in (zs @@ [z], aux)) (mbuf_t_empty, aux) (mebufn_add xss buf) 0 (nts @@ ts)
+    in (Rep_mbuf_t zs, MMatchP I mr mrs \<phi>s buf nts aux))"
+| "meeval n ts db (MMatchF I mr mrs \<phi>s buf nts t aux) =
+    (let (xss, \<phi>s) = map_split id (map (meeval n ts db) \<phi>s);
+      (aux, buf, nt, nts') = mebufnt_take (update_matchF n I mr mrs) aux (mebufn_add xss buf) t (nts @@ ts);
+      (zs, aux) = eval_matchF I mr nt aux
+    in (zs, MMatchF I mr mrs \<phi>s buf nts' nt aux))"
+  by pat_completeness auto
+
+lemma psize_snd_meeval: "meeval_dom (n, t, db, \<phi>) \<Longrightarrow> size (snd (meeval n t db \<phi>)) = size \<phi>"
+  apply (induct rule: meeval.pinduct)
+  apply (auto simp only: prod.inject meeval.psimps Let_def snd_conv meformula.size map_split_map id_o map_split_eq_Pair_iff size_list_map o_apply cong: size_list_cong split: prod.splits)
+    apply (metis snd_conv size_letpast_meeval)
+    apply simp
+  done
+
+lemma total_meeval: "All meeval_dom"
+  by (relation "measure (\<lambda>(_, _, _, \<phi>). size \<phi>)") (auto simp: termination_simp psize_snd_meeval)
+
+termination meeval
+  by (rule total_meeval)
+
+lemma meval_code[code]: "meval j n ts db (Rep_meformula \<phi>) = (let (zs, \<phi>') = meeval n ts db \<phi> in (zs, Rep_meformula \<phi>'))"
+proof (induction n ts db \<phi> rule: meeval.induct)
+  case (4 n ts db p m \<phi> \<psi> i buf)
+  have IH: "size \<psi> = size \<phi> \<Longrightarrow> meval j m ts db (Monitor_Impl.Rep_meformula \<psi>) =
+    (case meeval m ts db \<psi> of (zs, \<psi>') \<Rightarrow> (zs, Monitor_Impl.Rep_meformula \<psi>'))" for ts db \<psi>
+    using 4 by auto
+  show ?case
+    using 4(1) 4(2)[OF refl _ refl refl]
+    by (cases "letpast_meeval0 (meeval m) j i mbuf_t_empty (list_of_option buf) (p, m) ts db \<phi>")
+       (auto simp: letpast_meval_def mbuf_t_empty.rep_eq split: prod.splits
+        dest!: letpast_meval0_cong_f[where ?eval="meval j m" and ?eval'="meeval m" and \<phi>=\<phi>, OF IH size_Rep_meformula, simplified] letpast_meeval0)
+next
+  case (8 n ts db A_pos A_neg L buf)
+  have "map fst (map (meeval n ts db) L) = map fst (map (meval j n ts db) (map Monitor_Impl.Rep_meformula L))"
+    "map snd (map (meval j n ts db) (map Monitor_Impl.Rep_meformula L)) = map Monitor_Impl.Rep_meformula (map snd (map (meeval n ts db) L))"
+    by (auto dest: 8 split: prod.splits)
+  then show ?case
+    using 8
+    by (auto simp only: Let_def meval.simps meeval.simps mbufn_add Rep_meformula.simps mbuf_t_empty.rep_eq
+        split: prod.splits dest!: mebufn_take mbufn_take_app)
+next
+  case (17 n ts db I mr mrs \<phi>s buf nts aux)
+  have IH: "zs = zs' \<and> \<phi>s' = map Rep_meformula \<phi>s''" if
+    "map_split id (map (meval j n ts db) (map Rep_meformula \<phi>s)) = (zs, \<phi>s')"
+    "map_split id (map (meeval n ts db) \<phi>s) = (zs', \<phi>s'')" for zs zs' \<phi>s' \<phi>s''
+    using 17 that
+    by (induction \<phi>s arbitrary: zs zs' \<phi>s' \<phi>s'') (auto simp: comp_def split: prod.splits)
+  show ?case
+    using 17
+    by (auto simp only: meval.simps meeval.simps Rep_meformula.simps Let_def mbufn_add mbuf_t_empty.rep_eq mbuf_t_append.rep_eq
+        split: prod.splits dest!: mebufnt_take IH dest: mbufnt_take_app)
+next
+  case (18 n ts db I mr mrs \<phi>s buf nts t aux)
+  have IH: "zs = zs' \<and> \<phi>s' = map Rep_meformula \<phi>s''" if
+    "map_split id (map (meval j n ts db) (map Rep_meformula \<phi>s)) = (zs, \<phi>s')"
+    "map_split id (map (meeval n ts db) \<phi>s) = (zs', \<phi>s'')" for zs zs' \<phi>s' \<phi>s''
+    using 18 that
+    by (induction \<phi>s arbitrary: zs zs' \<phi>s' \<phi>s'') (auto simp: comp_def split: prod.splits)
+  show ?case
+    using 18
+    by (auto simp only: meval.simps meeval.simps Rep_meformula.simps Let_def mbufn_add mbuf_t_append.rep_eq
+        split: prod.splits dest!: mebufnt_take IH)
+qed (auto simp: mbuf2_add mbuf_t_empty.rep_eq mbuf_t_append.rep_eq
+    simp del: mprev_next.simps meprev_next.simps eval_since.simps eeval_since.simps
+    split: prod.splits dest!: mebuf2_take mebuf2t_take meprev_next eeval_since)
+
+end
+end
+
 section \<open>Instantiation of the generic algorithm and code setup\<close>
 
 (*
@@ -103,10 +714,13 @@ global_interpretation verimon_maux: maux valid_vmsaux init_vmsaux add_new_ts_vms
   add_new_table_vmsaux result_vmsaux valid_vmuaux init_vmuaux add_new_vmuaux length_vmuaux
   eval_vmuaux
   defines vminit0 = "maux.minit0 (init_vmsaux :: _ \<Rightarrow> event_data vmsaux) (init_vmuaux :: _ \<Rightarrow> event_data vmuaux) :: _ \<Rightarrow> Formula.formula \<Rightarrow> _"
+  and vmeinit0 = "maux.meinit0 (init_vmsaux :: _ \<Rightarrow> event_data vmsaux) (init_vmuaux :: _ \<Rightarrow> event_data vmuaux) :: _ \<Rightarrow> Formula.formula \<Rightarrow> _"
   and vminit = "maux.minit (init_vmsaux :: _ \<Rightarrow> event_data vmsaux) (init_vmuaux :: _ \<Rightarrow> event_data vmuaux) :: Formula.formula \<Rightarrow> _"
   and vminit_safe = "maux.minit_safe (init_vmsaux :: _ \<Rightarrow> event_data vmsaux) (init_vmuaux :: _ \<Rightarrow> event_data vmuaux) :: Formula.formula \<Rightarrow> _"
   and vmeval_since = "maux.eval_since add_new_ts_vmsaux join_vmsaux add_new_table_vmsaux (result_vmsaux :: _ \<Rightarrow> event_data vmsaux \<Rightarrow> event_data table)"
+  and vmeeval_since = "maux.eeval_since add_new_ts_vmsaux join_vmsaux add_new_table_vmsaux (result_vmsaux :: _ \<Rightarrow> event_data vmsaux \<Rightarrow> event_data table)"
   and vmeval = "maux.meval add_new_ts_vmsaux join_vmsaux add_new_table_vmsaux (result_vmsaux :: _ \<Rightarrow> event_data vmsaux \<Rightarrow> _) add_new_vmuaux (eval_vmuaux :: _ \<Rightarrow> _ \<Rightarrow> event_data vmuaux \<Rightarrow> _)"
+  and vmeeval = "maux.meeval add_new_ts_vmsaux join_vmsaux add_new_table_vmsaux (result_vmsaux :: _ \<Rightarrow> event_data vmsaux \<Rightarrow> _) add_new_vmuaux (eval_vmuaux :: _ \<Rightarrow> _ \<Rightarrow> event_data vmuaux \<Rightarrow> _)"
   and letpast_vmeval = "maux.letpast_meval add_new_ts_vmsaux join_vmsaux add_new_table_vmsaux (result_vmsaux :: _ \<Rightarrow> event_data vmsaux \<Rightarrow> _) add_new_vmuaux (eval_vmuaux :: _ \<Rightarrow> _ \<Rightarrow> event_data vmuaux \<Rightarrow> _)"
   and vmstep = "maux.mstep add_new_ts_vmsaux join_vmsaux add_new_table_vmsaux (result_vmsaux :: _ \<Rightarrow> event_data vmsaux \<Rightarrow> _) add_new_vmuaux (eval_vmuaux :: _ \<Rightarrow> _ \<Rightarrow> event_data vmuaux \<Rightarrow> _)"
   and vmsteps0_stateless = "maux.msteps0_stateless add_new_ts_vmsaux join_vmsaux add_new_table_vmsaux (result_vmsaux :: _ \<Rightarrow> event_data vmsaux \<Rightarrow> _) add_new_vmuaux (eval_vmuaux :: _ \<Rightarrow> _ \<Rightarrow> event_data vmuaux \<Rightarrow> _)"
@@ -120,10 +734,13 @@ global_interpretation verimon_maux: maux valid_vmsaux init_vmsaux add_new_ts_vms
 global_interpretation default_maux: maux valid_mmsaux "init_mmsaux :: _ \<Rightarrow> event_data mmsaux" add_new_ts_mmsaux gc_join_mmsaux add_new_table_mmsaux result_mmsaux
   valid_mmuaux "init_mmuaux :: _ \<Rightarrow> event_data mmuaux" add_new_mmuaux length_mmuaux eval_mmuaux'
   defines minit0 = "maux.minit0 (init_mmsaux :: _ \<Rightarrow> event_data mmsaux) (init_mmuaux :: _ \<Rightarrow> event_data mmuaux) :: _ \<Rightarrow> Formula.formula \<Rightarrow> _"
+  and meinit0 = "maux.meinit0 (init_mmsaux :: _ \<Rightarrow> event_data mmsaux) (init_mmuaux :: _ \<Rightarrow> event_data mmuaux) :: _ \<Rightarrow> Formula.formula \<Rightarrow> _"
   and minit = "maux.minit (init_mmsaux :: _ \<Rightarrow> event_data mmsaux) (init_mmuaux :: _ \<Rightarrow> event_data mmuaux) :: Formula.formula \<Rightarrow> _"
   and minit_safe = "maux.minit_safe (init_mmsaux :: _ \<Rightarrow> event_data mmsaux) (init_mmuaux :: _ \<Rightarrow> event_data mmuaux) :: Formula.formula \<Rightarrow> _"
   and meval_since = "maux.eval_since add_new_ts_mmsaux gc_join_mmsaux add_new_table_mmsaux (result_mmsaux :: _ \<Rightarrow> event_data mmsaux \<Rightarrow> event_data table)"
+  and meeval_since = "maux.eeval_since add_new_ts_mmsaux gc_join_mmsaux add_new_table_mmsaux (result_mmsaux :: _ \<Rightarrow> event_data mmsaux \<Rightarrow> event_data table)"
   and meval = "maux.meval add_new_ts_mmsaux gc_join_mmsaux add_new_table_mmsaux (result_mmsaux :: _ \<Rightarrow> event_data mmsaux \<Rightarrow> _) add_new_mmuaux (eval_mmuaux' :: _ \<Rightarrow> _ \<Rightarrow> event_data mmuaux \<Rightarrow> _)"
+  and meeval = "maux.meeval add_new_ts_mmsaux gc_join_mmsaux add_new_table_mmsaux (result_mmsaux :: _ \<Rightarrow> event_data mmsaux \<Rightarrow> _) add_new_mmuaux (eval_mmuaux' :: _ \<Rightarrow> _ \<Rightarrow> event_data mmuaux \<Rightarrow> _)"
   and letpast_meval = "maux.letpast_meval add_new_ts_mmsaux gc_join_mmsaux add_new_table_mmsaux (result_mmsaux :: _ \<Rightarrow> event_data mmsaux \<Rightarrow> _) add_new_mmuaux (eval_mmuaux' :: _ \<Rightarrow> _ \<Rightarrow> event_data mmuaux \<Rightarrow> _)"
   and mstep = "maux.mstep add_new_ts_mmsaux gc_join_mmsaux add_new_table_mmsaux (result_mmsaux :: _ \<Rightarrow> event_data mmsaux \<Rightarrow> _) add_new_mmuaux (eval_mmuaux' :: _ \<Rightarrow> _ \<Rightarrow> event_data mmuaux \<Rightarrow> _)"
   and msteps0_stateless = "maux.msteps0_stateless add_new_ts_mmsaux gc_join_mmsaux add_new_table_mmsaux (result_mmsaux :: _ \<Rightarrow> event_data mmsaux \<Rightarrow> _) add_new_mmuaux (eval_mmuaux' :: _ \<Rightarrow> _ \<Rightarrow> event_data mmuaux \<Rightarrow> _)"
@@ -153,17 +770,17 @@ lemma meval_pred_impl_eq: "meval_pred_impl n ts db e tms mode =
   unfolding meval_pred_impl_def
   by (force simp: Option.these_def image_iff intro!: option.case_cong pred_mode.case_cong)
 
-lemma meval_MPred: "meval lookahead n ts db (MPred e tms mode) =
-  (meval_pred_impl n ts db e tms mode, MPred e tms mode)"
+lemma meeval_MPred: "meeval lookahead n ts db (meformula.MPred e tms mode) =
+  (meval_pred_impl n ts db e tms mode, meformula.MPred e tms mode)"
   by (simp add: meval_pred_impl_eq)
 
-lemma vmeval_MPred: "vmeval lookahead n ts db (MPred e tms mode) =
-  (meval_pred_impl n ts db e tms mode, MPred e tms mode)"
+lemma vmeeval_MPred: "vmeeval lookahead n ts db (meformula.MPred e tms mode) =
+  (meval_pred_impl n ts db e tms mode, meformula.MPred e tms mode)"
   by (simp add: meval_pred_impl_eq)
 
-declare [[code drop: meval vmeval]]
-lemmas meval_code[code] = default_maux.meval_simps(1) meval_MPred default_maux.meval_simps(3-)
-lemmas vmeval_code[code] = verimon_maux.meval_simps(1) vmeval_MPred verimon_maux.meval_simps(3-)
+declare [[code drop: meeval vmeeval]]
+lemmas meeval_code[code] = default_maux.meeval.simps(1) meeval_MPred default_maux.meeval.simps(3-)
+lemmas vmeeval_code[code] = verimon_maux.meeval.simps(1) vmeeval_MPred verimon_maux.meeval.simps(3-)
 
 definition mk_db :: "((Formula.name \<times> nat) \<times> event_data option list set) list \<Rightarrow> database" where
   "mk_db m = Mapping.of_alist (map (\<lambda>(p, X). (p, [X])) m)"
@@ -599,35 +1216,6 @@ lemma Sup_rec_safety_atms[code_unfold]:
   by (simp add: Sup_rec_safety_def csorted_list_of_set_def ccompare_rec_safety_def ID_def
       linorder.set_sorted_list_of_set[OF comparator.linorder] comparator_rec_safety
       flip: comp_fun_idem_on.fold_set_fold[OF comp_fun_idem_on_sup])
-
-
-lift_definition MBuf2_t :: "'a queue \<Rightarrow> 'a mbuf_t" is "linearize" .
-
-code_datatype MBuf2_t
-
-lemma mbuf_t_empty_code[code]: "mbuf_t_empty = MBuf2_t empty_queue"
-  by transfer' (auto simp: empty_queue_rep)
-
-lemma mbuf_t_Cons_code[code]: "mbuf_t_Cons x (MBuf2_t xs) = MBuf2_t (prepend_queue x xs)"
-  by transfer' (auto simp: prepend_queue_rep)
-
-lemma mbuf_t_append_code[code]: "mbuf_t_append (MBuf2_t xs) ys = MBuf2_t (fold append_queue ys xs)"
-  apply transfer'
-  subgoal for xs ys
-  proof (induction ys arbitrary: xs)
-    case (Cons y ys)
-    show ?case
-      using Cons[of "append_queue y xs"]
-      by (auto simp: append_queue_rep)
-  qed simp
-  done
-
-lemma mbuf_t_is_empty_code[code]: "mbuf_t_is_empty (MBuf2_t xs) = is_empty xs"
-  by transfer' (auto simp: is_empty_alt)
-
-lemma mbuf_t_cases_code[code]: "mbuf_t_cases (MBuf2_t xs) = (case safe_hd xs of (None, xs') \<Rightarrow> (None, MBuf2_t xs')
-  | (Some x, xs') \<Rightarrow> (Some x, MBuf2_t (tl_queue xs')))"
-  by transfer' (auto simp: tl_queue_rep[unfolded is_empty_alt, OF list.discI] split: list.splits prod.splits option.splits dest: safe_hd_rep)
 
 (*<*)
 end
